coq/FcfLems.v
@@ -1,0 +1,164 @@
+Add LoadPath "~/fcf/src".
+Require Import Program FCF.FCF CpdtTactics.
+
+
+Lemma sumList_single : forall {A : Set} (x:A) (f : A -> Rat), sumList (x :: nil) f == f x.
+  unfold sumList; unfold fold_left; simpl.
+  intros;
+  rewrite <- ratAdd_0_l.
+  apply eqRat_refl.
+  Qed.
+
+Lemma unfold_repeat_true : forall {A : Set} (P : A -> bool) (C : Comp A) x, (P x) = true -> evalDist (Repeat C P) x == (evalDist C x) * ratInverse (sumList (filter P (getSupport C)) (evalDist C)).
+  intros.
+  crush.
+  unfold indicator.
+  crush.
+  rewrite ratMult_comm.
+  apply ratMult_eqRat_compat.
+  apply eqRat_refl.
+  rewrite ratMult_1_l.
+  apply eqRat_refl.
+Qed.
+
+Lemma unfold_repeat_false : forall {A : Set} (P : A -> bool) (C : Comp A) x, (P x) = false -> evalDist (Repeat C P) x == 0.
+  intros.
+  crush; unfold indicator; crush;
+    repeat rewrite ratMult_0_l; apply eqRat_refl.
+  Qed.
+ 
+Lemma repeat_in_support : forall {A : Set} (P : A -> bool) (C : Comp A) x, In x (getSupport (Repeat C P)) -> (P x) = true.
+  intros.
+  simpl in H.
+  apply filter_In in H.
+  crush.
+Qed.
+
+
+Definition negP {A : Set} (P : A -> bool) := fun x => negb (P x).
+
+Definition cond_prob {A : Set} (C : Comp A) (P : A -> bool) := sumList (filter P (getSupport C)) (evalDist C).
+
+Lemma cond_prob_Pr {A : Set} (C : Comp A) (P : A -> bool) : (cond_prob C P) == Pr [x <-$ C; ret ((P x) ?= true)].
+  admit. (*calculation about filter *)
+Admitted.
+
+
+Lemma ratMult_comm_assoc_r : forall a b c, a * (b * c) == a * (c * b).
+  intros;
+  apply ratMult_eqRat_compat;
+  [apply eqRat_refl |
+  apply ratMult_comm].
+Qed.
+
+Lemma ratMult_comm_assoc_l : forall a b c, (a * b) * c == (b * a) * c.
+  intros; apply ratMult_eqRat_compat;
+  [apply ratMult_comm | apply eqRat_refl].
+Qed.
+                                                                     
+Lemma repeat_split : forall {A : Set} (P : A -> bool) (C : Comp A), well_formed_comp (Repeat C P) -> well_formed_comp (Repeat C (negP P)) -> forall x, evalDist C x == (cond_prob C P) * (evalDist (Repeat C P) x) + (cond_prob C (negP P)) * (evalDist (Repeat C (negP P)) x).
+  intros.
+  crush.
+  unfold indicator, negP, negb, cond_prob.
+  destruct (P x);
+  repeat rewrite ratMult_0_l;
+  repeat rewrite ratMult_0_r;
+  try rewrite <- ratAdd_0_r.
+  rewrite ratMult_1_l.
+  rewrite <- ratMult_assoc.
+  rewrite ratMult_comm.
+  rewrite ratMult_comm_assoc_r.
+  rewrite ratInverse_prod_1.
+  rewrite ratMult_1_r; apply eqRat_refl.
+  admit. (* due to well formedness *)
+  rewrite <- ratAdd_0_l.
+  rewrite ratMult_1_l.
+  rewrite <- ratMult_assoc.
+  rewrite ratMult_comm.
+  rewrite ratMult_comm_assoc_r.
+  rewrite ratInverse_prod_1.
+  rewrite ratMult_1_r; apply eqRat_refl.
+  admit. (* due to well-formedness *)
+Admitted.
+
+Lemma filter_exists {A : Set} (l : list A) (P : A -> bool) : {l = nil} + {filter P l <> nil /\ ((filter (negP P) l) = nil)} + { filter P l = nil /\  (filter (negP P) l) <> nil } + {filter P l <> nil /\  (filter (negP P) l) <> nil}.
+  induction l.
+  left; left; left.
+  auto.
+  rewrite filter_cons.
+  remember (P a) as b.
+  assert (negP P a = negb b).
+  unfold negP; rewrite Heqb; auto.
+  unfold negb in H.
+  rewrite filter_cons; rewrite H.
+
+
+  destruct IHl.
+  destruct s.
+  destruct s.
+  destruct b; subst.
+  left; left; right; crush.
+  unfold filter.
+  left; right; crush.
+  destruct b; subst.
+  left; left; right; crush.
+  right; crush.
+  destruct b; subst.
+  right; crush.
+  left; right; crush.
+  destruct b; subst.
+  right; crush.
+  right; crush.
+Qed.
+
+
+
+Lemma if_repeat_decomp_ {A B : Set} `{EqDec A} `{EqDec B} (C : Comp A) (C1 C2 : A -> Comp B) (P : A -> bool) : (forall x, well_formed_comp (C1 x)) -> (forall x, well_formed_comp (C2 x)) -> well_formed_comp (Repeat C P) -> well_formed_comp (Repeat C (fun n => negb (P n))) -> forall a a', evalDist (x <-$ C; y <-$ (if (P x) then C1 x else C2 x); ret (x,y)) (a, a') == (Pr [x <-$ C; ret (P x)]) * (evalDist (x <-$ Repeat C P; y <-$ C1 x; ret (x,y)) (a, a')) + (Pr [x <-$ C; ret (negb (P x))]) * (evalDist (x <-$ Repeat C (fun n => negb (P n)); y <-$ C2 x; ret (x,y)) (a, a')).
+  intros.
+  rewrite (repeat_split (fun p => (P (fst p)))).
+  remember (P a) as b.
+  destruct b.
+  apply ratAdd_eqRat_compat.
+  apply ratMult_eqRat_compat.
+  rewrite cond_prob_Pr.
+  fcf_inline leftc.
+  comp_skip.
+  fcf_inline leftc.
+  remember (P x) as b; destruct b; subst.
+  fcf_irr_l.
+  simpl.
+  admit.
+  fcf_irr_l.
+  simpl.
+  admit.
+  admit.
+
+  apply ratMult_eqRat_compat.
+  rewrite cond_prob_Pr.
+  admit. (* similar *)
+
+  admit.
+  apply ratAdd_eqRat_compat.
+  apply ratMult_eqRat_compat.
+  admit.
+  admit.
+  apply ratMult_eqRat_compat.
+  admit.
+  admit.
+  admit. (* from H1 and H2 *)
+  admit. (* from H1 and H2 *)
+Admitted.
+
+
+Lemma if_repeat_decomp_both {A B : Set} `{EqDec A} `{EqDec B} (C : Comp A) (C1 C2 : A -> Comp B) (P : A -> bool) : (forall x, well_formed_comp (C1 x)) -> (forall x, well_formed_comp (C2 x)) -> well_formed_comp (Repeat C P) -> well_formed_comp (Repeat C (fun n => negb (P n))) -> forall a, evalDist (x <-$ C; (if (P x) then C1 x else C2 x)) a == (Pr [x <-$ C; ret (P x)]) * (evalDist (x <-$ Repeat C P; C1 x) a) + (Pr [x <-$ C; ret (negb (P x))]) * (evalDist (x <-$ Repeat C (fun n => negb (P n)); C2 x) a).
+  admit. (* follows from above *)
+Admitted.
+
+Lemma if_repeat_decomp_l {A B : Set} `{EqDec A} `{EqDec B} (C : Comp A) (C1 C2 : A -> Comp B) (P : A -> bool) : (forall x, well_formed_comp (C1 x)) -> well_formed_comp (Repeat C P) -> (cond_prob C (negP P)) == 0 -> forall a, evalDist (x <-$ C; (if (P x) then C1 x else C2 x)) a == (evalDist (x <-$ Repeat C P; C1 x) a) .
+  admit.
+  (* using unfold_repeat_true / false *)
+Admitted.
+
+Lemma if_repeat_decomp_r {A B : Set} `{EqDec A} `{EqDec B} (C : Comp A) (C1 C2 : A -> Comp B) (P : A -> bool) : (forall x, well_formed_comp (C1 x)) -> well_formed_comp (Repeat C (negP P)) -> (cond_prob C P) == 0 -> forall a, evalDist (x <-$ C; (if (P x) then C1 x else C2 x)) a == (evalDist (x <-$ Repeat C (negP P); C2 x) a) .
+  admit.
+Admitted.
